decompose_ is inverse of plug_

LambdaFDollar.v
@@ -29,28 +29,41 @@ Definition tm_dec (e : tm ␀) : (val ␀ + non ␀) :=
 Lemma tm_decide : ∀ e, (∃ v, tm_dec e = inl v) \/ (∃ p, tm_dec e = inr p).
 Proof.
   intro e; remember (tm_dec e) as d eqn: H; destruct d; solve [left + right; eexists; auto].
-  Qed.
-
+Qed.
 Lemma tm_dec_val : ∀ e v, tm_dec e = inl v → e = val_to_tm v.
 Proof.
   intros; inv e; cbn in *; try destruct a; inv H; auto.
-  Qed.
+Qed.
 Lemma tm_dec_non : ∀ e p, tm_dec e = inr p → e = non_to_tm p.
 Proof.
   intros; inv e; cbn in *; try destruct a; inv H; auto.
-  Qed.
+Qed.
+Lemma tm_dec_of_val : ∀ v, tm_dec (val_to_tm v) = inl v.
+Proof.
+  intros; destruct v; auto.
+Qed.
+Lemma tm_dec_of_non : ∀ p, tm_dec (non_to_tm p) = inr p.
+Proof.
+  intros; destruct p; auto.
+Qed.
 
-Ltac inv_tm_dec :=
+Ltac reason := repeat(
+  rewrite tm_dec_of_val in * +
+  rewrite tm_dec_of_non in * +
   match goal with
   | H : ␀ |- _ => destruct H
   | H : (_, _) = (_, _) |- _ => inj H
   | H : inl ?v = tm_dec ?e |- _ => rewrite (tm_dec_val e v (eq_sym H)) in *; auto
   | H : inr ?p = tm_dec ?e |- _ => rewrite (tm_dec_non e p (eq_sym H)) in *; auto
+  | H : context C [let (_, _) := ?e in _] |- _ =>
+    let p := fresh "p" in remember e as p; inv p
+  | |- context C [let (_, _) := ?e in _] => 
+    let p := fresh "p" in remember e as p; inv p
   | H : context C [match tm_dec ?e with inl _ => _ | inr _ => _ end] |- _ =>
     let td := fresh "td" in
     let Hd := fresh "Hd" in
     remember (tm_dec e) as td eqn: Hd; inv td; try rewrite Hd in *
-  end.
+  end).
 
 
 Section Contexts.
@@ -76,8 +89,8 @@ Section Contexts.
   Fixpoint plugT' trail e :=
     match trail with
     | T_nil' => e
-    | T_cons' v t => plugT' t <{ {val_to_tm v} $ e }>
-    (* | T_cons' v t => <{ {val_to_tm v} $ {plugT' t e} }> *)
+    (* | T_cons' v t => plugT' t <{ {val_to_tm v} $ e }> *)
+    | T_cons' v t => <{ {val_to_tm v} $ {plugT' t e} }>
     end.
 
   Definition redex_to_term' r := 
@@ -94,7 +107,7 @@ Arguments redex' A : clear implicits.
 Arguments dec' A : clear implicits.
 
 (* decompose:  T[w $ e]  into  T'[r]*)
-Fixpoint decompose'T (t : T' ␀) (w : val ␀) (e : tm ␀) : T' ␀ * redex' ␀ :=
+(* Fixpoint decompose'T (t : T' ␀) (w : val ␀) (e : tm ␀) : T' ␀ * redex' ␀ :=
   match e with
   | <{ var a }> => from_void a
   | <{ λ  e' }> => pair t (redex_dollar' w (val_abs e'))
@@ -112,6 +125,30 @@ Fixpoint decompose'T (t : T' ␀) (w : val ␀) (e : tm ␀) : T' ␀ * redex' �
     match tm_dec e1 with
     | inr p1 => pair t (redex_let' w (J_dol e2) p1)
     | inl v1 => decompose'T (T_cons' w t) v1 e2
+    end
+  end. *)
+
+(* decompose:  w $ e  into  T'[r]*)
+Fixpoint decompose'W (w : val ␀) (e : tm ␀) : T' ␀ * redex' ␀ :=
+  match e with
+  | <{ var a }> => from_void a
+  | <{ λ  e' }> => (T_nil', redex_dollar' w (val_abs e'))
+  | <{ S₀ e' }> => (T_nil', redex_shift'  w          e' )
+  | <{ e1 e2 }> =>
+    match tm_dec e1 with
+    | inr p1 => (T_nil', redex_let' w (J_fun e2) p1)
+    | inl v1 => 
+      match tm_dec e2 with
+      | inr p2 => (T_nil', redex_let' w (J_arg v1) p2)
+      | inl v2 => (T_cons' w T_nil', redex_beta' v1 v2)
+      end
+    end
+  | <{ e1 $ e2 }> => 
+    match tm_dec e1 with
+    | inr p1 => (T_nil', redex_let' w (J_dol e2) p1)
+    | inl v1 => 
+      let (t, r) := decompose'W v1 e2
+      in (T_cons' w t, r)
     end
   end.
 
@@ -135,8 +172,9 @@ Fixpoint decompose' (e : tm ␀) : dec' ␀ :=
     match decompose' e1 with
     | dec_stuck' k e'  => dec_stuck' (K_dol k e2) e'
     | dec_redex' k t r => dec_redex' (K_dol k e2) t r
-    | dec_value' v1    => 
-      let (t, r) := decompose'T T_nil' v1 e2 in
+    | dec_value' v1    =>
+      let (t, r) := decompose'W v1 e2 in
+      (* let (t, r) := decompose'T T_nil' v1 e2 in *)
       dec_redex' K_nil t r
     end
   end.
@@ -145,36 +183,36 @@ Ltac inv_decompose_match' H :=
   match goal with
   | H : (match decompose' ?e with | dec_stuck' _ _ | dec_redex' _ _ _ | dec_value' _ => _ end = _) |- _ =>
     let d := fresh "d" in remember (decompose' e) as d; inv d; inv_decompose_match' H
-  | H : (let (_,_) := decompose'T ?t ?w ?e in _) = _ |- _ =>
-    let d := fresh "d" in remember (decompose'T t w e) as d; inv d; inv_decompose_match' H
+  | H : (let (_,_) := ?e in _) = _ |- _ =>
+    let d := fresh "d" in remember e as d; inv d; inv_decompose_match' H
   | _ => try solve [inversion H; auto]; try inj H
   end.
 
 
-Lemma plug_dec : forall t (e : tm ␀),
-  (plugT' t e = e /\ t = T_nil') \/
-  (∃ t' v, plugT' t e = <{ {val_to_tm v} $ {plugT' t' e} }>).
-Proof.
-  induction t; intros.
-  left; auto.
-  right; cbn.
-  destruct (IHt <{ {val_to_tm v} $ e }>) as [[H H2]|[t' [v0 H]]]; subst; cbn in *.
-  exists T_nil'; eexists; eauto.
-  exists (T_cons' v t'); eexists. rewrite H. reflexivity.
-Qed.
+(* Lemma plug_dec : forall t (e : tm ␀),
+    (plugT' t e = e /\ t = T_nil') \/
+    (∃ t' v, plugT' t e = <{ {val_to_tm v} $ {plugT' t' e} }>).
+  Proof.
+    induction t; intros.
+    left; auto.
+    right; cbn.
+    destruct (IHt <{ {val_to_tm v} $ e }>) as [[H H2]|[t' [v0 H]]]; subst; cbn in *.
+    exists T_nil'; eexists; eauto.
+    exists (T_cons' v t'); eexists. rewrite H. reflexivity.
+  Qed.
 
-Lemma redex_plug_redex : ∀ t (r r' : redex' ␀),
-  redex_to_term' r = plugT' t (redex_to_term' r') →
-  t = T_nil'.
-Proof with cbn in *; auto.
-  intros. destruct (plug_dec t (redex_to_term' r')) as [ [H1 H2] | [t' [v H1]]]; subst; cbn in *; auto.
-  rewrite <- H in H1.
-  destruct r; cbn in *.
-  inv H1.
-  inv H1. admit.
-  inv H1. admit.
-  inv H1. admit.
-Admitted.
+  Lemma redex_plug_redex : ∀ t (r r' : redex' ␀),
+    redex_to_term' r = plugT' t (redex_to_term' r') →
+    t = T_nil'.
+  Proof with cbn in *; auto.
+    intros. destruct (plug_dec t (redex_to_term' r')) as [ [H1 H2] | [t' [v H1]]]; subst; cbn in *; auto.
+    rewrite <- H in H1.
+    destruct r; cbn in *.
+    inv H1.
+    inv H1. admit.
+    inv H1. admit.
+    inv H1. admit.
+  Admitted. *)
 
 Lemma inj_non : ∀ {A} (p p' : non A),
   non_to_tm p = non_to_tm p' → p = p'.
@@ -226,17 +264,31 @@ Ltac inv_dec' :=
   | H : dec_stuck' ?k ?e' = decompose' ?e |- _ => rewrite (decompose_stuck_inversion' e k e'); cbn; auto
   end.
 
-Lemma decomposeT_inversion' : ∀ t v e t' r,
+(* Lemma decomposeT_inversion' : ∀ t v e t' r,
   decompose'T t v e = (t', r) → 
   plugT' t <{ {val_to_tm v} $ e }> = plugT' t' (redex_to_term' r).
 Proof.
   intros t v e; generalize dependent v; generalize dependent t;
   dependent induction e; intros; cbn in *;
-  repeat inv_tm_dec; cbn;
+  reason; cbn;
   try solve [f_equal; auto].
   apply IHe2 in H; auto.
-  Qed.
+  Qed. *)
 
+Lemma decomposeW_j_p : ∀ w j p,
+  decompose'W w (plugJ j (non_to_tm p)) = (T_nil', redex_let' w j p).
+Proof.
+  intros; inv j; cbn; reason; reflexivity.
+Qed.
+Lemma decomposeW_inversion' : ∀ w e t r,
+  decompose'W w e = (t, r) →
+  <{ {val_to_tm w} $ e }> = plugT' t (redex_to_term' r).
+Proof.
+  intros w e; generalize dependent w;
+  dependent induction e; intros; cbn in *;
+  reason; cbn; f_equal.
+  apply IHe2; auto.
+Qed.
 Lemma decompose_redex_inversion' : ∀ e t k r,
   decompose' e = dec_redex' k t r → e = plugK k (plugT' t (redex_to_term' r)).
 Proof.
@@ -245,17 +297,15 @@ Proof.
   inv_decompose_match' H;
   repeat inv_dec'; cbn; f_equal;
   try solve [apply IHk + apply IHe1 + apply IHe2; auto].
-  erewrite <- (decomposeT_inversion' _ _ _ t r); eauto.
-  auto.
-  Qed.
-
+  (* erewrite <- (decomposeT_inversion' _ _ _ t r); eauto. *)
+  erewrite <- (decomposeW_inversion' _ _ t r); eauto.
+Qed.
 (* decompose' ∘ plug = id *)
 Lemma decompose_plug_value' : ∀ v,
   decompose' (val_to_tm v) = dec_value' v.
 Proof.
   intros; destruct v; auto.
-  Qed.
-
+Qed.
 Lemma decompose_plug_stuck' : ∀ k e, 
   decompose' (plugK k <{ S₀ e }>) = dec_stuck' k e.
 Proof.
@@ -264,43 +314,31 @@ Proof.
   - rewrite IHk; auto.
   - rewrite decompose_plug_value'. rewrite IHk; auto.
   - rewrite IHk; auto.
-  Qed.
-
+Qed.
+Lemma decomposeW_plug_redex : ∀ w t r,
+  decompose'W w (plugT' t (redex_to_term' r)) = ((T_cons' w t), r).
+Proof with cbn in *; auto.
+  intros w t; generalize dependent w; induction t; intros...
+  - inv r; cbn; reason; cbn in *;
+    try reflexivity.
+    + destruct v0... reason. reflexivity.
+    + rewrite decomposeW_j_p in Heqp. reason. reflexivity.
+  - reason. rewrite IHt in Heqp. reason. reflexivity.
+Qed.
 Lemma decompose_plug_redex' : ∀ k t r,
   decompose' (plugK k (plugT' t (redex_to_term' r))) = dec_redex' k t r.
-Proof with cbn in *; auto.
+Proof with cbn; auto.
   intros k t; generalize dependent k; induction t; intros...
   - induction k...
     + inv r; cbn; inv v; cbn; try solve [inv v0; auto]; auto.
-      match goal with
-      | |- context C [let (_,_) := ?e in _] => remember e as p eqn:H; destruct p
-      end.
-      symmetry in H. apply decomposeT_inversion' in H. cbn in H.
-      assert (<{ (λ t) $ {plugJ j (non_to_tm n)} }> = redex_to_term' (redex_let' (val_abs t) j n)) by auto.
-      rewrite H0 in H. apply redex_plug_redex in H as Hnil. subst. cbn in H. rewrite H0 in H. apply inj_redex in H. subst.
-      f_equal.
+      reason. rewrite decomposeW_j_p in Heqp. reason. reflexivity.
     + inv j; try inv v; cbn; try solve [rewrite IHk; auto].
   - induction k...
-    + cbn. inv v... rewrite IHt...
-    + inv j; try inv v0; cbn; try solve [rewrite IHk0; auto].
-  Qed.
+    + inv v... reason...
+      rewrite decomposeW_plug_redex in Heqp. reason. reflexivity.
+    + inv j; try inv v0; cbn; try solve [rewrite IHk; auto].
+Qed.
 
-(* Fixpoint decompose_e (k : K ␀) (e : tm ␀) : dec ␀ :=
-  match e with
-  | <{ var a }> => from_void a
-  | <{ λ  e' }> => decompose_K (val_abs e') k
-  | <{ S₀ e' }> => dec_stuck k e'
-  | <{ e1   e2 }> => decompose_e (K_fun k e2) e1
-  | <{ e1 $ e2 }> => decompose_e (K_dol k e2) e1
-  end
-with decompose_K (v : val ␀) (k : K ␀) : dec ␀ :=
-  match k with
-  | K_nil => dec_value v
-  | K_cons (J_fun e2) k1 => decompose_e (K_arg v k1) e2
-  | K_cons (J_arg v1) k2 => dec_redex k2 T_nil (redex_beta v1 v)
-  | K_cons (J_dol e2) k1 => todo
-  end
-. *)
 
 (* v $ K[p] ~> v' $ p *)
 (* Fixpoint decompose'K (v : val ␀) (k : K ␀) : val ␀.
